<?xml version="1.0"?>
<!-- This file is part of the book                    -->
<!--                                                  -->
<!-- Abstract Algebra: Theory and Applications        -->
<!--                                                  -->
<!-- Text: Copyright (C) 1997-2018  Thomas W. Judson  -->
<!-- Sage: Copyright (C) 2010-2018  Robert A. Beezer  -->
<!-- See the file COPYING for copying conditions.     -->
<!-- This file is part of the book                    -->
<!--                                                  -->
<!-- See the file COPYING for copying conditions.     -->
  <section xmlns:xi="http://www.w3.org/2001/XInclude" xml:id="section-cosets" permid="xMb">
      <title>Cosets</title>
      <p permid="oOb">
        Let <m>G</m> be a group and <m>H</m> a subgroup of <m>G</m>.
        Define a <term>left coset</term>
            <idx><h>Coset</h><h>left</h></idx>
        of <m>H</m> with <term>representative</term><idx><h>Coset</h><h>representative</h></idx> <m>g \in G</m> to be the set
        <me permid="ZFd">
          gH = \{ gh : h \in H \}
        </me>.
        <term>Right cosets</term>
            <idx><h>Coset</h><h>right</h></idx>
        can be defined similarly by
        <me permid="FMm">
          Hg = \{ hg : h \in H \}
        </me>.
        If left and right cosets coincide or if it is clear from the context to which type of coset that we are referring,
        we will use the word <em>coset</em>
        without specifying left or right.
      </p>

      <example xml:id="example-cosets-z6-cosets" permid="UdZ">
        <p permid="zIF">
          Let <m>H</m> be the subgroup of
          <m>{\mathbb Z}_6</m> consisting of the elements <m>0</m> and <m>3</m>.
          The cosets are
          <md permid="lTv">
            <mrow>0 + H = 3 + H = \{ 0, 3 \}</mrow>
            <mrow>1 + H = 4 + H = \{ 1, 4 \}</mrow>
            <mrow>2 + H = 5 + H = \{ 2, 5 \}</mrow>
          </md>.
          We will always write the cosets of subgroups of <m>{\mathbb Z}</m> and
          <m>{\mathbb Z}_n</m> with the additive notation we have used for cosets here.
          In a commutative group, left and right cosets are always identical.
        </p>
      </example>

      <example xml:id="example-cosets-s3-cosets" permid="Ali">
        <p permid="fPO">
          Let <m>H</m> be the subgroup of <m>S_3</m> defined by the permutations <m>\{(1), (123), (132) \}</m>.
          The left cosets of <m>H</m> are
          <md permid="SaE">
            <mrow>(1)H = (1 2 3)H =  (132)H = \{(1), (1 23), (132) \}</mrow>
            <mrow>(1 2)H = (1 3)H = (2 3)H =  \{ (1 2), (1 3), (2 3)  \}</mrow>
          </md>.
          The right cosets of <m>H</m> are exactly the same as the left cosets:
          <md permid="yhN">
            <mrow>H(1) = H(1 2 3) =  H(132) = \{(1), (1 23), (132) \}</mrow>
            <mrow>H(1 2) = H(1 3) = H(2 3) =  \{ (1 2), (1 3), (2 3)  \}</mrow>
          </md>.
        </p>

        <p permid="LWX">
          It is not always the case that a left coset is the same as a right coset.
          Let <m>K</m> be the subgroup of <m>S_3</m> defined by the permutations <m>\{(1), (1 2)\}</m>.
          Then the left cosets of <m>K</m> are
          <md permid="eoW">
            <mrow>(1)K = (1 2)K = \{(1), (1 2)\}</mrow>
            <mrow>(1 3)K = (1 2 3)K = \{(1 3), (1 2 3)\}</mrow>
            <mrow>(2 3)K = (1 3 2)K = \{(2 3), (1 3 2)\};</mrow>
          </md>
          however, the right cosets of <m>K</m> are
          <md permid="Kwf">
            <mrow>K(1) = K(1 2) = \{(1), (1 2)\}</mrow>
            <mrow>K(1 3) = K(1 3 2) = \{(1 3), (1 3 2)\}</mrow>
            <mrow>K(2 3) = K(1 2 3) = \{(2 3), (1 2 3)\}</mrow>
          </md>.
        </p>
      </example>

      <p permid="UVk">
        The following lemma is quite useful when dealing with cosets.
        (We leave its proof as an exercise.)
      </p>

      <lemma xml:id="lemma-cosets-theorem-1" permid="vBp">
        <statement>
          <p permid="bfV">
            Let <m>H</m> be a subgroup of a group <m>G</m> and suppose that <m>g_1, g_2 \in G</m>.
            The following conditions are equivalent.

            <ol permid="fWS">
              <li permid="ahG">
                <p permid="dMg">
                  <m>g_1 H = g_2 H</m>;
                </p>
              </li>

              <li permid="GoP">
                <p permid="JTp">
                  <m>H g_1^{-1} = H g_2^{-1}</m>;
                </p>
              </li>

              <li permid="mvY">
                <p permid="qay">
                  <m>g_1 H \subset g_2 H</m>;
                </p>
              </li>

              <li permid="SDh">
                <p permid="WhH">
                  <m>g_2 \in g_1 H</m>;
                </p>
              </li>

              <li permid="yKq">
                <p permid="CoQ">
                  <m>g_1^{-1} g_2 \in H</m>.
                </p>
              </li>
            </ol>
          </p>
        </statement>
      </lemma>

      <p permid="Bct">
        In all of our examples the cosets of a subgroup <m>H</m> partition the larger group <m>G</m>.
        The following theorem proclaims that this will always be the case.
      </p>

      <theorem xml:id="theorem-cosets-theorem-2" permid="SoM">
        <statement>
          <p permid="xTs">
            Let <m>H</m> be a subgroup of a group <m>G</m>.
            Then the left cosets of <m>H</m> in <m>G</m> partition <m>G</m>.
            That is, the group <m>G</m> is the disjoint union of the left cosets of <m>H</m> in <m>G</m>.
          </p>
        </statement>

        <proof permid="xqC">
          <p permid="ozG">
            Let <m>g_1 H</m> and <m>g_2 H</m> be two cosets of <m>H</m> in <m>G</m>.
            We must show that either <m>g_1 H \cap g_2 H = \emptyset</m> or <m>g_1 H = g_2 H</m>.
            Suppose that <m>g_1 H \cap g_2 H \neq \emptyset</m> and <m>a \in g_1 H \cap g_2 H</m>.
            Then by the definition of a left coset,
            <m>a = g_1 h_1 = g_2 h_2</m> for some elements <m>h_1</m> and <m>h_2</m> in <m>H</m>.
            Hence, <m>g_1 = g_2 h_2 h_1^{-1}</m> or <m>g_1 \in g_2 H</m>.
            By <xref ref="lemma-cosets-theorem-1"/>, <m>g_1 H = g_2 H</m>.
          </p>
        </proof>
      </theorem>

      <remark permid="sGJ">
        <p permid="Esy">
          There is nothing special in this theorem about left cosets.
          Right cosets also partition <m>G</m>;
          the proof of this fact is exactly the same as the proof for left cosets except that all group multiplications are done on the opposite side of <m>H</m>.
        </p>
      </remark>

      <p permid="hjC">
        Let <m>G</m> be a group and <m>H</m> be a subgroup of <m>G</m>.
        Define the <term>index</term>
            <idx><h>Index of a subgroup</h></idx>
            <idx><h>Subgroup</h><h>index of</h></idx>
        of <m>H</m> in <m>G</m> to be the number of left cosets of <m>H</m> in <m>G</m>.
        We will denote the index by <m>[G:H]</m>.

        <notation>
          <usage>[G:H]</usage>
          <description>index of a subgroup <m>H</m> in a group <m>G</m></description>
        </notation>

      </p>

      <example xml:id="example-cosets-z6-index" permid="gsr">
        <p permid="seg">
          Let <m>G= {\mathbb Z}_6</m> and <m>H = \{ 0, 3 \}</m>.
          Then <m>[G:H] = 3</m>.
        </p>
      </example>

      <example xml:id="example-cosets-s3-index" permid="MzA">
        <p permid="Ylp">
          Suppose that <m>G= S_3</m>,
          <m>H = \{ (1),(123), (132) \}</m>,
          and <m>K= \{ (1), (12) \}</m>.
          Then <m>[G:H] = 2</m> and <m>[G:K] = 3</m>.
        </p>
      </example>

      <theorem xml:id="theorem-cosets-theorem-3" permid="yvV">
        <statement>
          <p permid="eaB">
            Let <m>H</m> be a subgroup of a group <m>G</m>.
            The number of left cosets of <m>H</m> in <m>G</m> is the same as the number of right cosets of <m>H</m> in <m>G</m>.
          </p>
        </statement>

        <proof permid="dxL">
          <p permid="UGP">
            Let <m>{\mathcal L}_H</m> and
            <m>{\mathcal R}_H</m> denote the set of left and right cosets of <m>H</m> in <m>G</m>,
            respectively.

            <notation>
              <usage>\mathcal L_H</usage>
              <description>the set of left cosets of a subgroup <m>H</m> in a group <m>G</m></description>
            </notation>

            <notation>
              <usage>\mathcal R_H</usage>
              <description>the set of right cosets of a subgroup <m>H</m> in a group <m>G</m></description>
            </notation>

            If we can define a bijective map <m>\phi : {\mathcal L}_H \rightarrow {\mathcal R}_H</m>,
            then the theorem will be proved.
            If <m>gH \in {\mathcal L}_H</m>,
            let <m>\phi( gH ) = Hg^{-1}</m>.
            By <xref ref="lemma-cosets-theorem-1"/>, the map <m>\phi</m> is well-defined;
            that is, if <m>g_1 H = g_2 H</m>,
            then <m>H g_1^{-1} = H g_2^{-1}</m>.
            To show that <m>\phi</m> is one-to-one, suppose that
            <me permid="qDo">
              H g_1^{-1} = \phi( g_1 H ) = \phi( g_2 H ) = H g_2^{-1}
            </me>.
            Again by <xref ref="lemma-cosets-theorem-1"/>, <m>g_1 H = g_2 H</m>.
            The map <m>\phi</m> is onto since <m>\phi(g^{-1} H ) = H g</m>.
          </p>
        </proof>
      </theorem>
    </section>